src/lib/op_stats.cc
@@ -146,6 +146,7 @@ int op_stats::_send_stats(thread_pool* req_tp, thread_pool* other_tp, storage* s
 	_send_stat("get_hits" 						, stats_object->get_get_hits());
 	_send_stat("get_misses" 					, stats_object->get_get_misses());
 	_send_stat("delete_hits"					, stats_object->get_delete_hits());
+	_send_stat("proxy_write_dropped"	, stats_object->get_proxy_write_dropped());
 	_send_stat("delete_misses"				, stats_object->get_delete_misses());
 	_send_stat("incr_hits"						, stats_object->get_incr_hits());
 	_send_stat("incr_misses"					, stats_object->get_incr_misses());
